proof/iu_system/uni/algo_worklist/transfer.v
@@ -59,185 +59,185 @@ Proof.
     dependent destruction H4. auto.
 Qed. *)
 
-Inductive inst_typ : subst_set -> typ -> typ -> Prop := 
-  | inst_typ__tvar : forall θ X, 
+Inductive trans_typ : subst_set -> typ -> typ -> Prop := 
+  | trans_typ__tvar : forall θ X, 
       wf_ss θ -> 
       binds X (dbind_tvar_empty) θ ->
-      inst_typ θ (typ_var_f X) (typ_var_f X)
-  | inst_typ__stvar : forall θ X, 
+      trans_typ θ (typ_var_f X) (typ_var_f X)
+  | trans_typ__stvar : forall θ X, 
       wf_ss θ -> 
       binds X (dbind_stvar_empty) θ ->
-      inst_typ θ (typ_var_f X) (typ_var_f X)
-  | inst_typ__etvar : forall θ X A1,
+      trans_typ θ (typ_var_f X) (typ_var_f X)
+  | trans_typ__etvar : forall θ X A1,
       wf_ss θ ->
       binds X (dbind_typ A1) θ ->
-      inst_typ θ (typ_var_f X) A1
-  | inst_typ_unit : forall θ,
+      trans_typ θ (typ_var_f X) A1
+  | trans_typ_unit : forall θ,
       wf_ss θ ->
-      inst_typ θ typ_unit typ_unit
-  | inst_typ__bot : forall θ,
+      trans_typ θ typ_unit typ_unit
+  | trans_typ__bot : forall θ,
       wf_ss θ ->
-      inst_typ θ typ_bot typ_bot
-  | inst_typ__top : forall θ,
+      trans_typ θ typ_bot typ_bot
+  | trans_typ__top : forall θ,
       wf_ss θ ->
-      inst_typ θ typ_top typ_top
-  | inst_typ__arrow : forall θ A1ᵃ A2ᵃ A1ᵈ A2ᵈ,
-      inst_typ θ A1ᵃ A1ᵈ ->
-      inst_typ θ A2ᵃ A2ᵈ ->
-      inst_typ θ (typ_arrow A1ᵃ A2ᵃ) (typ_arrow A1ᵈ A2ᵈ)
-  | inst_typ__all : forall θ L A1ᵃ A1ᵈ,
+      trans_typ θ typ_top typ_top
+  | trans_typ__arrow : forall θ A1ᵃ A2ᵃ A1ᵈ A2ᵈ,
+      trans_typ θ A1ᵃ A1ᵈ ->
+      trans_typ θ A2ᵃ A2ᵈ ->
+      trans_typ θ (typ_arrow A1ᵃ A2ᵃ) (typ_arrow A1ᵈ A2ᵈ)
+  | trans_typ__all : forall θ L A1ᵃ A1ᵈ,
       (forall X, X `notin` L -> 
-        inst_typ ((X, dbind_tvar_empty) :: θ) (open_typ_wrt_typ A1ᵃ (typ_var_f X)) (open_typ_wrt_typ A1ᵈ (typ_var_f X))
+        trans_typ ((X, dbind_tvar_empty) :: θ) (open_typ_wrt_typ A1ᵃ (typ_var_f X)) (open_typ_wrt_typ A1ᵈ (typ_var_f X))
       ) ->
-      inst_typ θ (typ_all A1ᵃ) (typ_all A1ᵈ)
+      trans_typ θ (typ_all A1ᵃ) (typ_all A1ᵈ)
   | ins_typ__intersection : forall θ A1ᵃ A2ᵃ A1ᵈ A2ᵈ,
-      inst_typ θ A1ᵃ A1ᵈ ->
-      inst_typ θ A2ᵃ A2ᵈ ->
-      inst_typ θ (typ_intersection A1ᵃ A2ᵃ) (typ_intersection A1ᵈ A2ᵈ)
-  | inst_typ__union : forall θ A1ᵃ A2ᵃ A1ᵈ A2ᵈ,
-      inst_typ θ A1ᵃ A1ᵈ ->
-      inst_typ θ A2ᵃ A2ᵈ ->
-      inst_typ θ (typ_union A1ᵃ A2ᵃ) (typ_union A1ᵈ A2ᵈ)
+      trans_typ θ A1ᵃ A1ᵈ ->
+      trans_typ θ A2ᵃ A2ᵈ ->
+      trans_typ θ (typ_intersection A1ᵃ A2ᵃ) (typ_intersection A1ᵈ A2ᵈ)
+  | trans_typ__union : forall θ A1ᵃ A2ᵃ A1ᵈ A2ᵈ,
+      trans_typ θ A1ᵃ A1ᵈ ->
+      trans_typ θ A2ᵃ A2ᵈ ->
+      trans_typ θ (typ_union A1ᵃ A2ᵃ) (typ_union A1ᵈ A2ᵈ)
   . 
 
-Inductive inst_exp : subst_set -> exp -> exp -> Prop :=
-  | inst_exp__unit : forall θ,
+Inductive trans_exp : subst_set -> exp -> exp -> Prop :=
+  | trans_exp__unit : forall θ,
       wf_ss θ ->
-      inst_exp θ exp_unit exp_unit
-  | inst_exp__var : forall θ x,
+      trans_exp θ exp_unit exp_unit
+  | trans_exp__var : forall θ x,
       wf_ss θ ->
-      inst_exp θ (exp_var_f x) (exp_var_f x)
-  | inst_exp__abs : forall L θ eᵃ eᵈ,
+      trans_exp θ (exp_var_f x) (exp_var_f x)
+  | trans_exp__abs : forall L θ eᵃ eᵈ,
       (forall x, x `notin` L -> 
-        inst_exp θ (open_exp_wrt_exp eᵃ (exp_var_f x))
+        trans_exp θ (open_exp_wrt_exp eᵃ (exp_var_f x))
                    (open_exp_wrt_exp eᵈ (exp_var_f x))
         ) ->
-      inst_exp θ (exp_abs eᵃ) (exp_abs eᵈ)
-  | inst_exp__app : forall θ e1ᵃ e2ᵃ e1ᵈ e2ᵈ,
-      inst_exp θ e1ᵃ e1ᵈ ->
-      inst_exp θ e2ᵃ e2ᵈ ->
-      inst_exp θ (exp_app e1ᵃ e2ᵃ) (exp_app e1ᵈ e2ᵈ)
-  | inst_exp__tabs : forall L θ bᵃ bᵈ,
+      trans_exp θ (exp_abs eᵃ) (exp_abs eᵈ)
+  | trans_exp__app : forall θ e1ᵃ e2ᵃ e1ᵈ e2ᵈ,
+      trans_exp θ e1ᵃ e1ᵈ ->
+      trans_exp θ e2ᵃ e2ᵈ ->
+      trans_exp θ (exp_app e1ᵃ e2ᵃ) (exp_app e1ᵈ e2ᵈ)
+  | trans_exp__tabs : forall L θ bᵃ bᵈ,
       (forall X, X \notin L -> 
         inst_body ((X, dbind_tvar_empty) :: θ) 
                   (open_body_wrt_typ bᵃ (typ_var_f X))
                   (open_body_wrt_typ bᵈ (typ_var_f X))
       ) ->
-      inst_exp θ (exp_tabs bᵃ) (exp_tabs bᵈ)
-  | inst_exp__tapp : forall θ eᵃ eᵈ A1ᵃ A1ᵈ,
-      inst_exp θ eᵃ eᵈ ->
-      inst_typ θ A1ᵃ A1ᵈ ->
-      inst_exp θ (exp_tapp eᵃ A1ᵃ) (exp_tapp eᵈ A1ᵈ)
-  | inst_exp__anno : forall θ eᵃ eᵈ A1ᵃ A1ᵈ, 
-      inst_exp θ eᵃ eᵈ ->
-      inst_typ θ A1ᵃ A1ᵈ ->
-      inst_exp θ (exp_anno eᵃ A1ᵃ) (exp_anno eᵈ A1ᵈ) 
+      trans_exp θ (exp_tabs bᵃ) (exp_tabs bᵈ)
+  | trans_exp__tapp : forall θ eᵃ eᵈ A1ᵃ A1ᵈ,
+      trans_exp θ eᵃ eᵈ ->
+      trans_typ θ A1ᵃ A1ᵈ ->
+      trans_exp θ (exp_tapp eᵃ A1ᵃ) (exp_tapp eᵈ A1ᵈ)
+  | trans_exp__anno : forall θ eᵃ eᵈ A1ᵃ A1ᵈ, 
+      trans_exp θ eᵃ eᵈ ->
+      trans_typ θ A1ᵃ A1ᵈ ->
+      trans_exp θ (exp_anno eᵃ A1ᵃ) (exp_anno eᵈ A1ᵈ) 
 with inst_body : subst_set -> body -> body -> Prop :=
   | inst_body__anno : forall θ eᵃ eᵈ A1ᵃ A1ᵈ,
-      inst_exp θ eᵃ eᵈ ->
-      inst_typ θ A1ᵃ A1ᵈ ->
+      trans_exp θ eᵃ eᵈ ->
+      trans_typ θ A1ᵃ A1ᵈ ->
       inst_body θ (body_anno eᵃ A1ᵃ) (body_anno eᵈ A1ᵈ)
 .
 
-Inductive inst_cont : subst_set -> cont -> cont -> Prop :=
-  | inst_cont__infabs : forall θ cᵃ cᵈ,
-    inst_cont θ cᵃ cᵈ ->
-    inst_cont θ (cont_infabs cᵃ) (cont_infabs cᵈ)
-  | inst_cont__infabs_union : forall θ A1ᵃ A1ᵈ cᵃ cᵈ,
-    inst_typ θ A1ᵃ A1ᵈ ->
-    inst_cont θ cᵃ cᵈ ->
-    inst_cont θ (cont_infabsunion A1ᵃ cᵃ) (cont_infabsunion A1ᵈ cᵈ)
-  | inst_cont__infapp : forall θ eᵃ eᵈ cᵃ cᵈ,
-    inst_exp θ eᵃ eᵈ ->
-    inst_cont θ cᵃ cᵈ ->
-    inst_cont θ (cont_infapp eᵃ cᵃ) (cont_infapp eᵈ cᵈ)
-  | inst_cont__inftapp : forall θ A1ᵃ A1ᵈ cᵃ cᵈ,
-    inst_typ θ A1ᵃ A1ᵈ ->
-    inst_cont θ cᵃ cᵈ ->
-    inst_cont θ (cont_inftapp A1ᵃ cᵃ) (cont_inftapp A1ᵈ cᵈ)
-  | inst_cont__inftappunion : forall θ A1ᵃ A1ᵈ A2ᵃ A2ᵈ cᵃ cᵈ,
-    inst_typ θ A1ᵃ A1ᵈ ->
-    inst_typ θ A2ᵃ A2ᵈ ->
-    inst_cont θ cᵃ cᵈ ->
-    inst_cont θ (cont_inftappunion A1ᵃ A2ᵃ cᵃ) (cont_inftappunion A1ᵈ A2ᵈ cᵈ)
-  | inst_cont__unioninftapp : forall θ A1ᵃ A1ᵈ cᵃ cᵈ,
-    inst_typ θ A1ᵃ A1ᵈ ->
-    inst_cont θ cᵃ cᵈ ->
-    inst_cont θ (cont_unioninftapp A1ᵃ cᵃ) (cont_unioninftapp A1ᵈ cᵈ)
-  | inst_cont__unioninfabs : forall θ A1ᵃ A1ᵈ cᵃ cᵈ,
-    inst_typ θ A1ᵃ A1ᵈ ->
-    inst_cont θ cᵃ cᵈ ->
-    inst_cont θ (cont_unioninfabs A1ᵃ cᵃ) (cont_unioninfabs A1ᵈ cᵈ)    
-  | inst_cont__sub : forall θ A1ᵃ A1ᵈ,
-    inst_typ θ A1ᵃ A1ᵈ ->
-    inst_cont θ (cont_sub A1ᵃ) (cont_sub A1ᵈ)
+Inductive trans_cont : subst_set -> cont -> cont -> Prop :=
+  | trans_cont__infabs : forall θ cᵃ cᵈ,
+    trans_cont θ cᵃ cᵈ ->
+    trans_cont θ (cont_infabs cᵃ) (cont_infabs cᵈ)
+  | trans_cont__infabs_union : forall θ A1ᵃ A1ᵈ cᵃ cᵈ,
+    trans_typ θ A1ᵃ A1ᵈ ->
+    trans_cont θ cᵃ cᵈ ->
+    trans_cont θ (cont_infabsunion A1ᵃ cᵃ) (cont_infabsunion A1ᵈ cᵈ)
+  | trans_cont__infapp : forall θ eᵃ eᵈ cᵃ cᵈ,
+    trans_exp θ eᵃ eᵈ ->
+    trans_cont θ cᵃ cᵈ ->
+    trans_cont θ (cont_infapp eᵃ cᵃ) (cont_infapp eᵈ cᵈ)
+  | trans_cont__inftapp : forall θ A1ᵃ A1ᵈ cᵃ cᵈ,
+    trans_typ θ A1ᵃ A1ᵈ ->
+    trans_cont θ cᵃ cᵈ ->
+    trans_cont θ (cont_inftapp A1ᵃ cᵃ) (cont_inftapp A1ᵈ cᵈ)
+  | trans_cont__inftappunion : forall θ A1ᵃ A1ᵈ A2ᵃ A2ᵈ cᵃ cᵈ,
+    trans_typ θ A1ᵃ A1ᵈ ->
+    trans_typ θ A2ᵃ A2ᵈ ->
+    trans_cont θ cᵃ cᵈ ->
+    trans_cont θ (cont_inftappunion A1ᵃ A2ᵃ cᵃ) (cont_inftappunion A1ᵈ A2ᵈ cᵈ)
+  | trans_cont__unioninftapp : forall θ A1ᵃ A1ᵈ cᵃ cᵈ,
+    trans_typ θ A1ᵃ A1ᵈ ->
+    trans_cont θ cᵃ cᵈ ->
+    trans_cont θ (cont_unioninftapp A1ᵃ cᵃ) (cont_unioninftapp A1ᵈ cᵈ)
+  | trans_cont__unioninfabs : forall θ A1ᵃ A1ᵈ cᵃ cᵈ,
+    trans_typ θ A1ᵃ A1ᵈ ->
+    trans_cont θ cᵃ cᵈ ->
+    trans_cont θ (cont_unioninfabs A1ᵃ cᵃ) (cont_unioninfabs A1ᵈ cᵈ)    
+  | trans_cont__sub : forall θ A1ᵃ A1ᵈ,
+    trans_typ θ A1ᵃ A1ᵈ ->
+    trans_cont θ (cont_sub A1ᵃ) (cont_sub A1ᵈ)
 .
 
 
-Inductive inst_work : subst_set -> work -> work -> Prop :=
-  | inst_work__inf : forall Θ eᵃ eᵈ cᵃ cᵈ,
-      inst_exp Θ eᵃ eᵈ ->
-      inst_cont Θ cᵃ cᵈ ->
-      inst_work Θ (work_infer eᵃ cᵃ) (work_infer eᵈ cᵈ)
-  | inst_work__chk : forall Θ eᵃ eᵈ A1ᵃ A1ᵈ,
-      inst_exp Θ eᵃ eᵈ ->
-      inst_typ Θ A1ᵃ A1ᵈ ->
-      inst_work Θ (work_check eᵃ A1ᵃ) (work_check eᵈ A1ᵈ)
-  | inst_work__infabs : forall Θ A1ᵃ A1ᵈ  cᵃ cᵈ,
-      inst_typ Θ A1ᵃ A1ᵈ ->
-      inst_cont Θ cᵃ cᵈ ->
-      inst_work Θ (work_infabs A1ᵃ cᵃ ) (work_infabs A1ᵈ cᵈ)
-  | inst_work__infabsunion : forall Θ A1ᵃ A1ᵈ A2ᵃ A2ᵈ cᵃ cᵈ,
-      inst_typ Θ A1ᵃ A1ᵈ ->
-      inst_typ Θ A2ᵃ A2ᵈ ->
-      inst_cont Θ cᵃ cᵈ ->
-      inst_work Θ (work_infabsunion A1ᵃ A2ᵃ cᵃ) (work_infabsunion A1ᵈ A2ᵈ cᵈ)
-  | inst_work__infapp : forall Θ A1ᵃ A1ᵈ eᵃ eᵈ cᵃ cᵈ,
-      inst_typ Θ A1ᵃ A1ᵈ ->
-      inst_exp Θ eᵃ eᵈ ->
-      inst_cont Θ cᵃ cᵈ ->
-      inst_work Θ (work_infapp A1ᵃ eᵃ cᵃ) (work_infapp A1ᵈ eᵈ cᵈ)
-  | inst_work__inftapp : forall Θ A1ᵃ A1ᵈ A2ᵃ A2ᵈ cᵃ cᵈ,
-      inst_typ Θ A1ᵃ A1ᵈ ->
-      inst_typ Θ A2ᵃ A2ᵈ ->
-      inst_cont Θ cᵃ cᵈ ->
-      inst_work Θ (work_inftapp A1ᵃ A2ᵃ cᵃ) (work_inftapp A1ᵈ A2ᵈ cᵈ)
-  | inst_work__sub : forall θ A1ᵃ A1ᵈ B1ᵃ B1ᵈ,
-      inst_typ θ A1ᵃ A1ᵈ ->
-      inst_typ θ B1ᵃ B1ᵈ ->
-      inst_work θ (work_sub A1ᵃ B1ᵃ) (work_sub A1ᵈ B1ᵈ)
-  | inst_work__inftappunion : forall Θ A1ᵃ A1ᵈ A2ᵃ A2ᵈ B1ᵃ B1ᵈ cᵃ cᵈ,
-      inst_typ Θ A1ᵃ A1ᵈ ->
-      inst_typ Θ A2ᵃ A2ᵈ ->
-      inst_typ Θ B1ᵃ B1ᵈ ->
-      inst_cont Θ cᵃ cᵈ ->
-      inst_work Θ (work_inftappunion A1ᵃ A2ᵃ B1ᵃ cᵃ) (work_inftappunion A1ᵈ A2ᵈ B1ᵈ cᵈ)
-  | inst_work__unioninftapp : forall Θ A1ᵃ A1ᵈ A2ᵃ A2ᵈ cᵃ cᵈ,
-      inst_typ Θ A1ᵃ A1ᵈ ->
-      inst_typ Θ A2ᵃ A2ᵈ ->
-      inst_cont Θ cᵃ cᵈ ->
-      inst_work Θ (work_unioninftapp A1ᵃ A2ᵃ cᵃ) (work_unioninftapp A1ᵈ A2ᵈ cᵈ)
-  | inst_work__unioninfabs : forall Θ A1ᵃ A1ᵈ A2ᵃ A2ᵈ cᵃ cᵈ,
-      inst_typ Θ A1ᵃ A1ᵈ ->
-      inst_typ Θ A2ᵃ A2ᵈ ->
-      inst_cont Θ cᵃ cᵈ ->
-      inst_work Θ (work_unioninfabs A1ᵃ A2ᵃ cᵃ) (work_unioninfabs A1ᵈ A2ᵈ cᵈ)
-  | inst_work__applycont : forall θ cᵃ cᵈ A1ᵃ A1ᵈ,
-      inst_cont θ cᵃ cᵈ ->
-      inst_typ θ A1ᵃ A1ᵈ ->
-      inst_work θ (work_apply cᵃ A1ᵃ) (work_apply cᵈ A1ᵈ)
+Inductive trans_work : subst_set -> work -> work -> Prop :=
+  | trans_work__inf : forall Θ eᵃ eᵈ cᵃ cᵈ,
+      trans_exp Θ eᵃ eᵈ ->
+      trans_cont Θ cᵃ cᵈ ->
+      trans_work Θ (work_infer eᵃ cᵃ) (work_infer eᵈ cᵈ)
+  | trans_work__chk : forall Θ eᵃ eᵈ A1ᵃ A1ᵈ,
+      trans_exp Θ eᵃ eᵈ ->
+      trans_typ Θ A1ᵃ A1ᵈ ->
+      trans_work Θ (work_check eᵃ A1ᵃ) (work_check eᵈ A1ᵈ)
+  | trans_work__infabs : forall Θ A1ᵃ A1ᵈ  cᵃ cᵈ,
+      trans_typ Θ A1ᵃ A1ᵈ ->
+      trans_cont Θ cᵃ cᵈ ->
+      trans_work Θ (work_infabs A1ᵃ cᵃ ) (work_infabs A1ᵈ cᵈ)
+  | trans_work__infabsunion : forall Θ A1ᵃ A1ᵈ A2ᵃ A2ᵈ cᵃ cᵈ,
+      trans_typ Θ A1ᵃ A1ᵈ ->
+      trans_typ Θ A2ᵃ A2ᵈ ->
+      trans_cont Θ cᵃ cᵈ ->
+      trans_work Θ (work_infabsunion A1ᵃ A2ᵃ cᵃ) (work_infabsunion A1ᵈ A2ᵈ cᵈ)
+  | trans_work__infapp : forall Θ A1ᵃ A1ᵈ eᵃ eᵈ cᵃ cᵈ,
+      trans_typ Θ A1ᵃ A1ᵈ ->
+      trans_exp Θ eᵃ eᵈ ->
+      trans_cont Θ cᵃ cᵈ ->
+      trans_work Θ (work_infapp A1ᵃ eᵃ cᵃ) (work_infapp A1ᵈ eᵈ cᵈ)
+  | trans_work__inftapp : forall Θ A1ᵃ A1ᵈ A2ᵃ A2ᵈ cᵃ cᵈ,
+      trans_typ Θ A1ᵃ A1ᵈ ->
+      trans_typ Θ A2ᵃ A2ᵈ ->
+      trans_cont Θ cᵃ cᵈ ->
+      trans_work Θ (work_inftapp A1ᵃ A2ᵃ cᵃ) (work_inftapp A1ᵈ A2ᵈ cᵈ)
+  | trans_work__sub : forall θ A1ᵃ A1ᵈ B1ᵃ B1ᵈ,
+      trans_typ θ A1ᵃ A1ᵈ ->
+      trans_typ θ B1ᵃ B1ᵈ ->
+      trans_work θ (work_sub A1ᵃ B1ᵃ) (work_sub A1ᵈ B1ᵈ)
+  | trans_work__inftappunion : forall Θ A1ᵃ A1ᵈ A2ᵃ A2ᵈ B1ᵃ B1ᵈ cᵃ cᵈ,
+      trans_typ Θ A1ᵃ A1ᵈ ->
+      trans_typ Θ A2ᵃ A2ᵈ ->
+      trans_typ Θ B1ᵃ B1ᵈ ->
+      trans_cont Θ cᵃ cᵈ ->
+      trans_work Θ (work_inftappunion A1ᵃ A2ᵃ B1ᵃ cᵃ) (work_inftappunion A1ᵈ A2ᵈ B1ᵈ cᵈ)
+  | trans_work__unioninftapp : forall Θ A1ᵃ A1ᵈ A2ᵃ A2ᵈ cᵃ cᵈ,
+      trans_typ Θ A1ᵃ A1ᵈ ->
+      trans_typ Θ A2ᵃ A2ᵈ ->
+      trans_cont Θ cᵃ cᵈ ->
+      trans_work Θ (work_unioninftapp A1ᵃ A2ᵃ cᵃ) (work_unioninftapp A1ᵈ A2ᵈ cᵈ)
+  | trans_work__unioninfabs : forall Θ A1ᵃ A1ᵈ A2ᵃ A2ᵈ cᵃ cᵈ,
+      trans_typ Θ A1ᵃ A1ᵈ ->
+      trans_typ Θ A2ᵃ A2ᵈ ->
+      trans_cont Θ cᵃ cᵈ ->
+      trans_work Θ (work_unioninfabs A1ᵃ A2ᵃ cᵃ) (work_unioninfabs A1ᵈ A2ᵈ cᵈ)
+  | trans_work__applycont : forall θ cᵃ cᵈ A1ᵃ A1ᵈ,
+      trans_cont θ cᵃ cᵈ ->
+      trans_typ θ A1ᵃ A1ᵈ ->
+      trans_work θ (work_apply cᵃ A1ᵃ) (work_apply cᵈ A1ᵈ)
 .
 
 
 Reserved Notation "θ ⫦ Ω ⇝ Γ ⫣ θ'"
   (at level 65, Ω at next level, Γ at next level, no associativity).
-Inductive inst_worklist : subst_set -> aworklist -> dworklist -> subst_set -> Prop := 
+Inductive trans_worklist : subst_set -> aworklist -> dworklist -> subst_set -> Prop := 
   | inst_wl__empty : forall θ, 
       wf_ss θ -> 
       θ ⫦ aworklist_empty ⇝ dworklist_empty ⫣ θ
   | inst_wl__conswork : forall θ θ' Γ Ω  wᵃ wᵈ, 
       θ ⫦ Γ ⇝ Ω ⫣ θ' ->
-      inst_work θ' wᵃ wᵈ ->
+      trans_work θ' wᵃ wᵈ ->
       θ ⫦ aworklist_conswork Γ wᵃ ⇝ dworklist_conswork Ω wᵈ ⫣ θ'
   | inst_wl__cons_tvar : forall θ θ' Γ Ω X, 
       θ ⫦ Γ ⇝ Ω ⫣ θ' ->
@@ -247,23 +247,23 @@ Inductive inst_worklist : subst_set -> aworklist -> dworklist -> subst_set -> Pr
       θ ⫦ aworklist_constvar Γ X abind_stvar_empty ⇝ dworklist_constvar Ω X dbind_stvar_empty ⫣  (X, dbind_stvar_empty) :: θ'
   | inst_wl__cons_var : forall θ θ' Γ Ω A1ᵃ A1ᵈ x, 
       θ ⫦ Γ ⇝ Ω ⫣ θ' ->
-      inst_typ θ' A1ᵃ A1ᵈ ->
+      trans_typ θ' A1ᵃ A1ᵈ ->
       θ ⫦ aworklist_consvar Γ x (abind_typ A1ᵃ) ⇝ dworklist_consvar Ω x (dbind_typ A1ᵈ) ⫣ θ'
   | inst_wl_ev : forall θ θ' Γ Ω Aᵃ Aᵈ Bᵃ Bᵈ T X, 
       θ ⫦ Γ ⇝ Ω ⫣ θ' -> 
-      inst_typ θ' Aᵃ Aᵈ ->
-      inst_typ θ' Bᵃ Bᵈ ->
+      trans_typ θ' Aᵃ Aᵈ ->
+      trans_typ θ' Bᵃ Bᵈ ->
       d_mono_typ (ss_to_denv θ' ) T ->
       dwl_to_denv Ω ⊢ Aᵈ <: T ->
       dwl_to_denv Ω ⊢ T <: Bᵈ ->
       θ ⫦ aworklist_constvar Γ X (abind_bound Aᵃ Bᵃ) ⇝ Ω ⫣  (X, dbind_typ T) :: θ'
-where "θ ⫦ Γᵃ ⇝ Γᵈ ⫣ θ'" := (inst_worklist θ Γᵃ Γᵈ θ').
+where "θ ⫦ Γᵃ ⇝ Γᵈ ⫣ θ'" := (trans_worklist θ Γᵃ Γᵈ θ').
 
-Hint Constructors inst_typ : Hdb_transfer.
+Hint Constructors trans_typ : Hdb_transfer.
 
 
 
-Lemma inst_work_not_in_ss : forall θ Γ Ω X,
+Lemma trans_work_not_in_ss : forall θ Γ Ω X,
   nil ⫦ Γ ⇝ Ω ⫣ θ -> X ∉ dom (awl_to_aenv Γ) -> X ∉ dom θ.
 Proof with auto.
   intros. dependent induction H; simpl in *...
@@ -297,19 +297,19 @@ Lemma a_wf_wl_wf_ss : forall θ Γ Ω,
   ⊢ᵃ Γ -> nil ⫦ Γ ⇝ Ω ⫣ θ -> wf_ss θ.
 Proof with eauto.
   intros. dependent induction H0; dependent destruction H...
-  - econstructor... eapply inst_work_not_in_ss...
-  - econstructor... eapply inst_work_not_in_ss...
-  - econstructor... eapply inst_work_not_in_ss... 
+  - econstructor... eapply trans_work_not_in_ss...
+  - econstructor... eapply trans_work_not_in_ss...
+  - econstructor... eapply trans_work_not_in_ss... 
 Qed.
 
 
 Hint Resolve a_wf_wl_wf_ss : Hdb_transfer.
 
-Notation "θ ⫦ᵗ Aᵃ ⇝ Aᵈ" := (inst_typ θ Aᵃ Aᵈ)
+Notation "θ ⫦ᵗ Aᵃ ⇝ Aᵈ" := (trans_typ θ Aᵃ Aᵈ)
   (at level 65, Aᵃ at next level, no associativity).
 
 
-Lemma inst_typ_det : forall θ Aᵃ A₁ᵈ A₂ᵈ,
+Lemma trans_typ_det : forall θ Aᵃ A₁ᵈ A₂ᵈ,
   uniq θ -> 
   θ ⫦ᵗ Aᵃ ⇝ A₁ᵈ -> 
   θ ⫦ᵗ Aᵃ ⇝ A₂ᵈ -> 
@@ -323,32 +323,25 @@ Proof with eauto with Hdb_transfer.
   - exfalso. eapply wf_ss_etvar_stvar_false... 
   - specialize (binds_unique _ _ _ _ _ H1 H3 H). intros.
     dependent destruction H4... 
-  - specialize (IHinst_typ1 H _ H2_).
-    specialize (IHinst_typ2 H _ H2_0).
+  - specialize (IHtrans_typ1 H _ H2_).
+    specialize (IHtrans_typ2 H _ H2_0).
     subst...
   - inst_cofinites_by (L `union` L0 `union` (ftvar_in_typ A1ᵈ) `union` (ftvar_in_typ A1ᵈ0) `union`  dom θ) using_name X.  
     apply f_equal.
     + eapply open_typ_wrt_typ_inj with (X1:=X); auto.
-  - specialize (IHinst_typ1 H _ H2_).
-    specialize (IHinst_typ2 H _ H2_0).
+  - specialize (IHtrans_typ1 H _ H2_).
+    specialize (IHtrans_typ2 H _ H2_0).
     subst...
-  - specialize (IHinst_typ1 H _ H2_).
-    specialize (IHinst_typ2 H _ H2_0).
+  - specialize (IHtrans_typ1 H _ H2_).
+    specialize (IHtrans_typ2 H _ H2_0).
     subst...
 Qed.
 
 
-Theorem a_mono_typ_wf : forall aE A,
-  a_mono_typ aE A -> a_wf_typ aE A.
-Proof.
-  intros. induction H; auto.
-  eapply a_wf_typ__etvar; eauto.
-Qed.
-
-Hint Constructors inst_typ : Hdb_transfer.
-Hint Constructors inst_cont : Hdb_transfer.
-Hint Constructors inst_work : Hdb_transfer.
-Hint Constructors inst_worklist : Hdb_transfer.
+Hint Constructors trans_typ : Hdb_transfer.
+Hint Constructors trans_cont : Hdb_transfer.
+Hint Constructors trans_work : Hdb_transfer.
+Hint Constructors trans_worklist : Hdb_transfer.
 Hint Constructors wf_ss : Hdb_transfer.
 
 
@@ -389,11 +382,11 @@ Qed.
 
 Lemma a_wf_typ_trans_typ : forall θ Γ Ω Aᵃ,
   a_wf_typ (awl_to_aenv Γ) Aᵃ ->  ⊢ᵃ Γ -> nil ⫦ Γ ⇝ Ω ⫣ θ -> exists Aᵈ,
-    inst_typ θ Aᵃ Aᵈ.
+    trans_typ θ Aᵃ Aᵈ.
 Proof with eauto with Hdb_transfer.
   intros. dependent induction H...
   - exists (` X). econstructor... admit.
-  - exists (` X). eapply inst_typ__stvar... admit. 
+  - exists (` X). eapply trans_typ__stvar... admit. 
   - admit.
   - admit.
   - admit.
@@ -437,12 +430,12 @@ Proof with eauto with Hdb_transfer.
       * admit.
     + dependent destruction Hinst.
       * econstructor. admit. admit.
-      * eapply inst_typ__stvar. admit. admit.
+      * eapply trans_typ__stvar. admit. admit.
       * econstructor.
         admit.
         admit.
   - dependent destruction Hinst.
-    eapply inst_typ__all with (L:=L `union` singleton X). intros.
+    eapply trans_typ__all with (L:=L `union` singleton X). intros.
     inst_cofinites_with X0.
     rewrite typ_subst_open_comm...
     rewrite_env (((X0, dbind_tvar_empty) :: θ') ++ θ).
@@ -474,27 +467,12 @@ Proof with auto with Hdb_transfer.
       rewrite <- wf_subst_set_strength_etvar_same_denv...
 Qed.
 
-(* 
 
-Lemma inst_typ_rev_subst' : forall θ T X Aᵃ A'ᵈ,
-  lc_typ Aᵃ -> 
-  X `notin` dom θ ->
-  (ss_to_denv θ) ⊢ T ->
-  θ ⫦ᵗ {T /ᵗ X} Aᵃ ⇝ A'ᵈ -> 
-  exists Aᵈ, {T /ᵗ X} Aᵈ = A'ᵈ /\ (X, dbind_typ T) :: θ ⫦ᵗ Aᵃ ⇝ Aᵈ.
-Proof with eauto with Hdb_transfer.
-  intros * Hlc Hfv Hwft Hinst.
-  generalize dependent A'ᵈ.
-  dependent induction Hlc; simpl in *; intros.
-  - dependent destruction Hinst. 
-    exists typ_unit... intuition... econstructor... *)
 
 Hint Resolve wf_subst_set_strength_etvar : Hdb_transfer.
 
 
-(* Lemma inst_typ_weaken  *)
-
-Lemma inst_typ_rename : forall θ1 θ2 Aᵃ Aᵈ X X', 
+Lemma trans_typ_rename : forall θ1 θ2 Aᵃ Aᵈ X X', 
   θ2 ++ (X, dbind_tvar_empty) :: θ1 ⫦ᵗ Aᵃ ⇝ Aᵈ ->
   map (subst_tvar_in_dbind (` X') X) θ2  ++ (X', dbind_tvar_empty) :: θ1 ⫦ᵗ {` X' /ᵗ X} Aᵃ ⇝ {` X' /ᵗ X} Aᵈ.
 Proof with auto with Hdb_transfer.
@@ -511,7 +489,7 @@ Proof with auto with Hdb_transfer.
   - econstructor... admit.
   - econstructor... admit.
   - econstructor... admit.
-  - eapply inst_typ__all with (L := L `union` singleton X).
+  - eapply trans_typ__all with (L := L `union` singleton X).
     intros. inst_cofinites_with X0.
     rewrite typ_subst_open_comm...
     rewrite typ_subst_open_comm...
@@ -519,17 +497,27 @@ Proof with auto with Hdb_transfer.
     eapply H0...
 Admitted.
 
-Corollary inst_typ_rename_cons : forall θ Aᵃ Aᵈ X X', 
+Corollary trans_typ_rename_cons : forall θ Aᵃ Aᵈ X X', 
   (X, dbind_tvar_empty) :: θ ⫦ᵗ Aᵃ ⇝ Aᵈ ->
   (X', dbind_tvar_empty) :: θ ⫦ᵗ {` X' /ᵗ X} Aᵃ ⇝ {` X' /ᵗ X} Aᵈ.
 Proof.
   intros. 
   rewrite_env (map (subst_tvar_in_dbind (` X') X) nil  ++ (X', dbind_tvar_empty) :: θ).
-  eapply inst_typ_rename. auto.
+  eapply trans_typ_rename. auto.
 Qed.
 
 
-
+Lemma in_ss_denv_in_ss : forall X b θ,
+  binds X b (ss_to_denv θ) ->
+  binds X b θ.
+Proof with auto with Hdb_transfer.
+  intros. induction θ...
+  - destruct a. destruct d...
+    + inversion H... 
+      dependent destruction H0...
+    + inversion H... 
+      dependent destruction H0...
+Qed.
 
 
 Lemma wf_ss_etvar_tvar : forall θ1 θ2 T X,
@@ -551,37 +539,58 @@ Admitted.
 Hint Resolve wf_ss_etvar_tvar : Hdb_transfer.
 
 
-Lemma inst_typ_weaken : forall θ1 θ2 θ3 Aᵃ Aᵈ,
+Lemma trans_typ_weaken : forall θ1 θ2 θ3 Aᵃ Aᵈ,
   θ3 ++ θ1 ⫦ᵗ Aᵃ ⇝ Aᵈ ->
   wf_ss (θ3 ++ θ2 ++ θ1) ->
   (θ3 ++ θ2 ++ θ1) ⫦ᵗ Aᵃ ⇝ Aᵈ.
 Proof with eauto with Hdb_transfer.
   intros. generalize dependent θ2.
   dependent induction H; intros...
-  - inst_cofinites_for inst_typ__all. intros.
+  - inst_cofinites_for trans_typ__all. intros.
     inst_cofinites_with X.
     rewrite_env (((X, ▫) :: θ3) ++ θ2 ++ θ1).
     eapply H0; simpl...
 Qed.
 
 
-Lemma inst_typ_refl: forall θ A,
+Lemma trans_typ_refl: forall θ A,
   ss_to_denv θ ⊢ A ->
   wf_ss θ ->
   θ ⫦ᵗ A ⇝ A.
 Proof with eauto with Hdb_transfer.
   intros. dependent induction H...
   - econstructor... admit.
-  - eapply inst_typ__stvar... admit.
+  - eapply trans_typ__stvar... admit.
   - econstructor. admit.
 Admitted.
 
 
-Lemma inst_typ_etvar_tvar_subst : forall θ1 θ2 T X Aᵃ A'ᵈ,
+Lemma etvar_bind_no_etvar: forall θ X A T,
+  wf_ss θ ->
+  ss_to_denv θ ⊢ A ->
+  binds X (dbind_typ T) θ ->
+  X \notin ftvar_in_typ A.
+Proof with eauto with Hdb_transfer.
+  intros. dependent induction H0...
+  + destruct (X == X0)...
+    subst. apply in_ss_denv_in_ss in H0.
+    exfalso. eapply wf_ss_etvar_tvar_false...
+  + destruct (X == X0)...
+    subst. apply in_ss_denv_in_ss in H0.
+    exfalso. eapply wf_ss_etvar_stvar_false...
+  + inst_cofinites_by (L `union` dom θ `union` singleton X) using_name X.
+    simpl.
+    rewrite ftvar_in_typ_open_typ_wrt_typ_lower.
+    eapply H1 with (θ:=(X0 ~ dbind_tvar_empty ++ θ))...
+    econstructor...
+Qed.
+
+
+Lemma trans_typ_etvar_tvar_subst : forall θ1 θ2 T X Aᵃ A'ᵈ,
   lc_typ Aᵃ -> 
   X `notin` dom (θ2 ++ θ1) ->
   d_mono_typ (ss_to_denv θ1) T ->
-  θ2 ++ (X, dbind_typ T) :: θ1 ⫦ᵗ {T /ᵗ X} Aᵃ ⇝ A'ᵈ -> 
+  θ2 ++ (X, dbind_typ T) :: θ1 ⫦ᵗ Aᵃ ⇝ A'ᵈ -> 
   exists Aᵈ, {T /ᵗ X} Aᵈ = A'ᵈ /\ θ2 ++ (X, dbind_tvar_empty) :: θ1 ⫦ᵗ Aᵃ ⇝ Aᵈ.
 Proof with eauto with Hdb_transfer.
   intros * Hlc Hfv Hwft Hinst.
@@ -597,10 +606,9 @@ Proof with eauto with Hdb_transfer.
     + subst. exists (` X0). split.
       * simpl. unfold eq_dec. destruct (EqDec_eq_of_X X0 X0).
         -- subst.
-           eapply inst_typ_det with (θ:=(θ2 ++ (X0, dbind_typ T) :: θ1)); eauto.
+           eapply trans_typ_det with (θ:=(θ2 ++ (X0, dbind_typ T) :: θ1)); eauto.
            admit.
-           eapply inst_typ_refl...
-           admit. admit.
+           admit. 
         -- contradiction.
       * econstructor... admit.
     + dependent destruction Hinst.
@@ -617,7 +625,6 @@ Proof with eauto with Hdb_transfer.
     intuition... subst...
   - dependent destruction Hinst.  
     pick fresh X0. inst_cofinites_with X0.
-    rewrite typ_subst_open_comm in H1...
     rewrite_env (((X0, dbind_tvar_empty) :: θ2) ++ (X, dbind_typ T) :: θ1) in H1.
     apply H0 in H1...
     destruct H1 as [Aᵈ].
@@ -625,11 +632,11 @@ Proof with eauto with Hdb_transfer.
     rewrite subst_tvar_in_typ_close_typ_wrt_typ... 
     split.
     + apply f_equal. erewrite typ_open_r_close_l... intuition.
-    + eapply inst_typ__all with (L:=L); intros.
+    + eapply trans_typ__all with (L:=L); intros.
       intuition.
       erewrite subst_tvar_in_typ_intro by auto.
       erewrite (subst_tvar_in_typ_intro X0 (close_typ_wrt_typ X0 Aᵈ)) by apply close_typ_notin.
-      apply inst_typ_rename_cons...
+      apply trans_typ_rename_cons...
       rewrite open_typ_wrt_typ_close_typ_wrt_typ...
   - dependent destruction Hinst.
     apply IHHlc1 in Hinst1... destruct Hinst1 as [A1'ᵈ]. 
@@ -644,18 +651,21 @@ Proof with eauto with Hdb_transfer.
 Admitted.
 
 
-Lemma inst_typ_etvar_tvar_subst_cons : forall θ1 T X Aᵃ A'ᵈ,
+Lemma trans_typ_etvar_tvar_subst_cons : forall θ1 T X Aᵃ A'ᵈ,
   lc_typ Aᵃ -> 
   X `notin` dom θ1 ->
   d_mono_typ (ss_to_denv θ1) T ->
   (X, dbind_typ T) :: θ1 ⫦ᵗ Aᵃ ⇝ A'ᵈ -> 
   exists Aᵈ, {T /ᵗ X} Aᵈ = A'ᵈ /\ (X, dbind_tvar_empty) :: θ1 ⫦ᵗ Aᵃ ⇝ Aᵈ.
-Proof.
-Admitted.
+Proof with auto with Hdb_transfer. 
+  intros. 
+  rewrite_env (nil ++ (X, ▫) :: θ1).  
+  apply trans_typ_etvar_tvar_subst...
+Qed.
 
 
-(* Hint Constructors inst_typ : transfer.
-Hint Constructors inst_worklist : transfer.
+(* Hint Constructors trans_typ : transfer.
+Hint Constructors trans_worklist : transfer.
 
 Lemma fv_ss_ld_ctx_dom: forall θ x,
   x `notin` fv_ss θ -> x `notin` ld_ctx_dom (ss_to_ctx θ).
@@ -728,33 +738,10 @@ Proof.
   intros; apply notin_union; auto.
 Qed.
 
-Lemma inst_wf : forall θ tᵃ tᵈ,
-  θ ⫦ tᵃ ⇝ tᵈ -> wf_ss θ.
-Proof.
-  intros. induction H; auto.
-  - inst_cofinites_by L. auto.
-Qed.
-
-Lemma inst_e_rev_subst : forall A'ᵈ θ tᵃ tᵈ x Aᵃ,
-  lc_la_type Aᵃ ->
-  x `notin` (fx_la_type tᵃ `union` fv_ss θ) -> 
-  θ ⫦ tᵃ ⇝ tᵈ → θ ⫦ [tᵃ /ᵃ x] Aᵃ ⇝ A'ᵈ ->
-  exists Aᵈ, [tᵈ /ᵗ x] Aᵈ = A'ᵈ ∧ θ ⫦ Aᵃ ⇝ Aᵈ.
-Proof.
-  intros.  
-  specialize (inst_e_rev_subst' _ _ _ _  _ H H0 H1 A'ᵈ).
-  intros.
-  specialize (H3 H2).
-  auto.
-Qed.
-
-*)
-
-
 (* Lemma transfer_reorder: forall Γᵃ Γ'ᵈ θ' x t m Γ'ᵃ,
   reorder Γᵃ x t m la_wl_nil Γ'ᵃ ->
-  inst_worklist nil Γ'ᵃ Γ'ᵈ θ' ->
-  exists Γᵈ θ, inst_worklist nil Γᵃ Γᵈ θ.
+  trans_worklist nil Γ'ᵃ Γ'ᵈ θ' ->
+  exists Γᵈ θ, trans_worklist nil Γᵃ Γᵈ θ.
 Proof.
   intros. 
   generalize dependent θ'.
@@ -783,8 +770,8 @@ Admitted.
 
 Lemma transfer_reorder': forall Γᵃ Γᵈ θ x t m Γ'ᵃ,
   reorder Γᵃ x t m la_wl_nil Γ'ᵃ ->
-  inst_worklist nil Γᵃ Γᵈ θ -> 
-  exists Γ'ᵈ θ', inst_worklist nil Γ'ᵃ Γ'ᵈ θ'.
+  trans_worklist nil Γᵃ Γᵈ θ -> 
+  exists Γ'ᵈ θ', trans_worklist nil Γ'ᵃ Γ'ᵈ θ'.
 Proof.
   intros. 
   generalize dependent θ.
@@ -812,8 +799,8 @@ Proof.
     + admit.
     + admit.
   - dependent destruction H0.
-Admitted. *)
-
+Admitted. 
+*)*)
 
 Definition transfer (Γ : aworklist) (Ω : dworklist)  : Prop :=
-  exists θ', inst_worklist nil Γ Ω θ'.
+  exists θ', trans_worklist nil Γ Ω θ'.
